Library/RandomTrait.dfy
@@ -1,0 +1,34 @@
+/*******************************************************************************
+ *  Copyright by the contributors to the Dafny Project
+ *  SPDX-License-Identifier: MIT
+ *******************************************************************************/
+
+// RUN: %verify "%s"
+
+include "Model/RandomNumberGenerator.dfy"
+include "Model/Model.dfy"
+
+module RandomTrait {
+  import opened RandomNumberGenerator
+  import Model
+
+  trait {:termination false} RandomTrait {
+    ghost var s: RNG
+
+    method Coin() returns (b: bool)
+      ensures Model.Coin(old(s)) == (b, s)
+
+    method Uniform(n: nat) returns (u: nat)
+      requires 0 < n
+      ensures Model.Uniform(n)(old(s)) == (u, s)
+
+    method UniformInterval(a: int, b: int) returns (u: int)
+      requires a < b
+      ensures Model.UniformInterval(a, b)(old(s)) == (u, s)
+
+    method Bernoulli(p: real) returns (c: bool) 
+      decreases *            
+      requires 0.0 <= p <= 1.0
+      ensures Model.Bernoulli(p)(old(s)) == (c, s) 
+  }
+}
